model/agp32StateScript.sml
@@ -2,18 +2,19 @@ open hardwarePreamble;
 
 val _ = new_theory "agp32State";
 
-val _ = Datatype `
-   IF_state = <| (** fetch related **)
-                 IF_PC_input: word32;
-                 IF_PC_output: word32;
-                 IF_instr: word32;
-                 IF_PC_write_enable: bool;
-                 PC_sel: word2 
-               |>`;
+(** IF_state: fetch related **)
+Datatype:
+  IF_state = <| IF_PC_input: word32;
+                IF_PC_output: word32;
+                IF_instr: word32;
+                IF_PC_write_enable: bool;
+                PC_sel: word2
+             |>
+End
 
-val _ = Datatype `
-   ID_state = <| (** decode related **)
-                 ID_PC: word32;
+(** ID_state: decode related **)
+Datatype:
+   ID_state = <| ID_PC: word32;
                  ID_instr: word32;
                  ID_read_dataA: word32;
                  ID_read_dataB: word32;
@@ -42,11 +43,12 @@ val _ = Datatype `
                  ID_addrW: word6;
                  ID_opc: word6;
                  ID_func: word4
-               |>`;
+              |>
+End
 
-val _ = Datatype `
-   EX_state = <| (** execute related **)
-                 EX_PC: word32;
+(** EX_state: execute related **)
+Datatype:
+   EX_state = <| EX_PC: word32;
                  EX_dataA: word32;
                  EX_dataB: word32;
                  EX_dataW: word32;
@@ -79,34 +81,36 @@ val _ = Datatype `
                  EX_addrW: word6;
                  EX_opc: word6;
                  EX_func: word4
-               |>`;
+              |>
+End
 
-val _ = Datatype `
-   MEM_state = <| (** memory related **)
-                 MEM_PC: word32;
-                 MEM_dataA: word32;
-                 MEM_dataB: word32;
-                 MEM_dataW: word32;
-                 MEM_imm: word32;
-                 MEM_imm_updated: word32;
-                 MEM_ALU_res: word32;
-                 MEM_SHIFT_res: word32;
-                 MEM_write_enable: bool;
-                 MEM_read_mem: bool;
-                 MEM_write_mem: bool;
-                 MEM_write_mem_byte: bool;
-                 MEM_write_reg: bool;
-                 MEM_isInterrupt: bool;
-                 MEM_state_flag: bool;
-                 MEM_NOP_flag: bool;
-                 MEM_enable: bool;
-                 MEM_addrW: word6;
-                 MEM_opc: word6 
-               |>`;
+(** MEM_state: memory related **)
+Datatype:
+   MEM_state = <| MEM_PC: word32;
+                  MEM_dataA: word32;
+                  MEM_dataB: word32;
+                  MEM_dataW: word32;
+                  MEM_imm: word32;
+                  MEM_imm_updated: word32;               
+                  MEM_ALU_res: word32;           
+                  MEM_SHIFT_res: word32;             
+                  MEM_write_enable: bool;                  
+                  MEM_read_mem: bool;            
+                  MEM_write_mem: bool;              
+                  MEM_write_mem_byte: bool;                
+                  MEM_write_reg: bool;            
+                  MEM_isInterrupt: bool;          
+                  MEM_state_flag: bool;
+                  MEM_NOP_flag: bool;             
+                  MEM_enable: bool;           
+                  MEM_addrW: word6;            
+                  MEM_opc: word6               
+               |>
+End
 
-val _ = Datatype `
-   WB_state = <| (** write back related **)
-                 WB_PC: word32;
+(** WB_state: write back related **)
+Datatype:
+   WB_state = <| WB_PC: word32;
                  WB_dataA: word32;
                  WB_read_data: word32;
                  WB_read_data_byte: word32;
@@ -122,40 +126,40 @@ val _ = Datatype `
                  WB_data_sel: word3;
                  WB_addrW: word6;
                  WB_opc: word6
-               |>`;
+              |>
+End
 
-val _ = Datatype `
-   state_circuit = 
-               <|(* pipelined Silver CPU *)
+(* pipelined Silver CPU *)
+Datatype:
+  state_circuit = <| (** globel state **)
+    state: word3;
+    PC: word32;
+    R: word6 -> word32;
+    data_out: word10;
+    data_in: word2;
+    acc_arg: word32;
+    acc_arg_ready: bool;
+    interrupt_req: bool;
+    do_interrupt: bool;
 
-                 (** globel state **)
-                 state: word3;
-                 PC: word32;
-                 R: word6 -> word32;
-                 data_out: word10;
-                 data_in: word2;
-                 acc_arg: word32;
-                 acc_arg_ready: bool;
-                 interrupt_req: bool;
-                 do_interrupt: bool;
+    (** memory(cache) interface **)
+    command: word3;
+    data_addr: word32;
+    data_wdata: word32;
+    data_wstrb: word4;
 
-                 (** data memory interface **)
-                 command: word3;
-                 data_addr: word32;
-                 data_wdata: word32;
-                 data_wstrb: word4;
+    (** accelerator **)
+    acc_res: word32;
+    acc_res_ready: bool;
+    acc_state: word2;
 
-                 (** accelerator **)
-                 acc_res: word32;
-                 acc_res_ready: bool;
-                 acc_state: word2;
-
-                 (** piepeline **)
-                 IF: IF_state;
-                 ID: ID_state;
-                 EX: EX_state;
-                 MEM: MEM_state;
-                 WB: WB_state 
-               |>`;
+    (** piepeline **)
+    IF: IF_state;
+    ID: ID_state;
+    EX: EX_state;
+    MEM: MEM_state;
+    WB: WB_state
+  |>
+End
 
 val _ = export_theory ();
